Added mutation proof

dev/lf/tight-proof/Definitions.v
@@ -1,6 +1,6 @@
 Set Implicit Arguments.
 
-Require Import LibLN.
+Require Import LibMap LibLN.
 Require Import Coq.Program.Equality.
 
 (* ###################################################################### *)
@@ -13,6 +13,8 @@ Require Import Coq.Program.Equality.
 Parameter typ_label: Set.
 Parameter trm_label: Set.
 
+Definition addr := var.
+
 Inductive label: Set :=
 | label_typ: typ_label -> label
 | label_trm: trm_label -> label.
@@ -24,6 +26,7 @@ Inductive avar : Set :=
 Inductive typ : Set :=
   | typ_top  : typ
   | typ_bot  : typ
+  | typ_ref  : typ -> typ (* Ref T *)
   | typ_rcd  : dec -> typ (* { D } *)
   | typ_and  : typ -> typ -> typ
   | typ_sel  : avar -> typ_label -> typ (* x.L *)
@@ -39,9 +42,13 @@ Inductive trm : Set :=
   | trm_sel  : avar -> trm_label -> trm
   | trm_app  : avar -> avar -> trm
   | trm_let  : trm -> trm -> trm (* let x = t in u *)
+  | trm_ref  : avar -> typ -> trm (* ref x T *)
+  | trm_deref  : avar -> trm (* !x *)
+  | trm_asg  : avar -> avar -> trm (* x := y *)
 with val : Set :=
   | val_new  : typ -> defs -> val
   | val_lambda : typ -> trm -> val
+  | val_loc : addr -> val
 with def : Set :=
   | def_typ  : typ_label -> typ -> def
   | def_trm  : trm_label -> trm -> def
@@ -52,8 +59,18 @@ with defs : Set :=
 (** *** Typing environment ("Gamma") *)
 Definition ctx := env typ.
 
-(** *** Value environment ("store") *)
-Definition sto := env val.
+(** *** Store typing ("Sigma") *)
+Definition sigma := env typ.
+
+(** *** Value environment ("sta") *)
+Definition stack := env val.
+
+(** *** Store ("sto") *)
+Definition store := LibMap.map addr var.
+
+Definition bindsM l x sto := LibBag.binds (A:=addr) (B:=var) sto l x.
+
+Definition emptyM : store := (@empty_impl addr var).
 
 (* ###################################################################### *)
 (** ** Definition list membership *)
@@ -93,6 +110,7 @@ Fixpoint open_rec_typ (k: nat) (u: var) (T: typ): typ :=
   match T with
   | typ_top        => typ_top
   | typ_bot        => typ_bot
+  | typ_ref T      => typ_ref (open_rec_typ k u T)
   | typ_rcd D      => typ_rcd (open_rec_dec k u D)
   | typ_and T1 T2  => typ_and (open_rec_typ k u T1) (open_rec_typ k u T2)
   | typ_sel x L    => typ_sel (open_rec_avar k u x) L
@@ -112,11 +130,15 @@ Fixpoint open_rec_trm (k: nat) (u: var) (t: trm): trm :=
   | trm_sel v m    => trm_sel (open_rec_avar k u v) m
   | trm_app f a    => trm_app (open_rec_avar k u f) (open_rec_avar k u a)
   | trm_let t1 t2  => trm_let (open_rec_trm k u t1) (open_rec_trm (S k) u t2)
+  | trm_ref a t    => trm_ref (open_rec_avar k u a) (open_rec_typ k u t)
+  | trm_deref a    => trm_deref (open_rec_avar k u a)
+  | trm_asg l r    => trm_asg (open_rec_avar k u l) (open_rec_avar k u r)
   end
 with open_rec_val (k: nat) (u: var) (v: val): val :=
   match v with
-  | val_new T ds => val_new (open_rec_typ (S k) u T) (open_rec_defs (S k) u ds)
+  | val_new T ds   => val_new (open_rec_typ (S k) u T) (open_rec_defs (S k) u ds)
   | val_lambda T e => val_lambda (open_rec_typ k u T) (open_rec_trm (S k) u e)
+  | val_loc n      => val_loc n
   end
 with open_rec_def (k: nat) (u: var) (d: def): def :=
   match d with
@@ -182,6 +204,7 @@ Fixpoint fv_typ (T: typ) : vars :=
   match T with
   | typ_top        => \{}
   | typ_bot        => \{}
+  | typ_ref T      => (fv_typ T)
   | typ_rcd D      => (fv_dec D)
   | typ_and T U    => (fv_typ T) \u (fv_typ U)
   | typ_sel x L    => (fv_avar x)
@@ -201,11 +224,15 @@ Fixpoint fv_trm (t: trm) : vars :=
   | trm_sel x m      => (fv_avar x)
   | trm_app f a      => (fv_avar f) \u (fv_avar a)
   | trm_let t1 t2    => (fv_trm t1) \u (fv_trm t2)
+  | trm_ref a t      => (fv_avar a) \u (fv_typ t)
+  | trm_deref a      => (fv_avar a)
+  | trm_asg l r      => (fv_avar l) \u (fv_avar r)
   end
 with fv_val (v: val) : vars :=
   match v with
   | val_new T ds    => (fv_typ T) \u (fv_defs ds)
   | val_lambda T e  => (fv_typ T) \u (fv_trm e)
+  | val_loc n       => \{}
   end
 with fv_def (d: def) : vars :=
   match d with
@@ -218,165 +245,198 @@ with fv_defs(ds: defs) : vars :=
   | defs_cons tl d   => (fv_defs tl) \u (fv_def d)
   end.
 
-Definition fv_ctx_types(G: ctx): vars := (fv_in_values (fun T => fv_typ T) G).
+Definition fv_env_types(e: env typ): vars := (fv_in_values (fun T => fv_typ T) e).
 
 (* ###################################################################### *)
 (** ** Operational Semantics *)
 
-Inductive red : trm -> sto -> trm -> sto -> Prop :=
-| red_sel : forall x m s t T ds,
-    binds x (val_new T ds) s ->
+Inductive red : trm -> stack -> store -> trm -> stack -> store -> Prop :=
+| red_sel : forall x m sta sto t T ds,
+    binds x (val_new T ds) sta ->
     defs_has (open_defs x ds) (def_trm m t) ->
-    red (trm_sel (avar_f x) m) s t s
-| red_app : forall f a s T t,
-    binds f (val_lambda T t) s ->
-    red (trm_app (avar_f f) (avar_f a)) s (open_trm a t) s
-| red_let : forall v t s x,
-    x # s ->
-    red (trm_let (trm_val v) t) s (open_trm x t) (s & x ~ v)
-| red_let_var : forall t s x,
-    red (trm_let (trm_var (avar_f x)) t) s (open_trm x t) s
-| red_let_tgt : forall t0 t s t0' s',
-    red t0 s t0' s' ->
-    red (trm_let t0 t) s (trm_let t0' t) s'.
+    red (trm_sel (avar_f x) m) sta sto t sta sto
+| red_app : forall f a sta sto T t,
+    binds f (val_lambda T t) sta ->
+    red (trm_app (avar_f f) (avar_f a)) sta sto (open_trm a t) sta sto
+| red_let : forall v t sta sto x,
+    x # sta ->
+    red (trm_let (trm_val v) t) sta sto (open_trm x t) (sta & x ~ v) sto
+| red_let_var : forall t sta sto x,
+    red (trm_let (trm_var (avar_f x)) t) sta sto (open_trm x t) sta sto
+| red_let_tgt : forall t0 t sta sto t0' sta' sto',
+    red t0 sta sto t0' sta' sto' ->
+    red (trm_let t0 t) sta sto (trm_let t0' t) sta' sto'
+| red_ref_var : forall x sta sto l T,
+    l \notindom sto ->
+    red (trm_ref (avar_f x) T) sta sto (trm_val (val_loc l)) sta sto[l :=  x]
+| red_asgn : forall x y l sta sto,
+    binds x (val_loc l) sta ->
+    l \indom sto -> (* TODO is this redundant? *)
+    red (trm_asg (avar_f x) (avar_f y)) sta sto (trm_var (avar_f y)) sta sto[l := y]
+| red_deref : forall x y (l: addr) sta (sto: store),
+    binds x (val_loc l) sta ->
+    bindsM l y sto ->
+    red (trm_deref (avar_f x)) sta sto (trm_var (avar_f y)) sta sto.
 
 (* ###################################################################### *)
 (** ** Typing *)
 
-(* todo: get rid of tymode and submode entirely by defining separate typing relations for
-   ty_trm (general typing), ty_trm_t (tight typing), and ty_trm_p (precise typing).
-   The best way to do this is to define them in the order
-   1) ty_trm
-   2) ty_trm_p
-   3) ty_trm_t
-   so that they can depend on each other without needing mutual recursion.
-   If the proof somewhere is defined for both general and tight, or both general and precise,
-   we could do the following:
-   - start by proving everything only for the most general typing
-   - if the prove somewhere depends on having a lemma for tight/precise typing, but we proved it only for general
-     typing, then you could
-     * modify the statement of the lemma to apply for tight/precise typing; the proof should be easy to change
-     * add a short lemma that proves the same for general typing
-     * the proof of that lemma should work by invoking the original tight version of the lemma, plus
-       tight-to-general. *)
 Inductive tymode: Set := ty_precise | ty_general.
 Inductive submode: Set := sub_tight | sub_general.
 
-Reserved Notation "G '|-' t '::' T" (at level 40, t at level 59).
-
-Inductive ty_trm : tymode -> submode -> ctx -> trm -> typ -> Prop :=
-| ty_var : forall m1 m2 G x T,
+Inductive ty_trm : tymode -> submode -> ctx -> sigma -> trm -> typ -> Prop :=
+| ty_var : forall m1 m2 G S x T,
     binds x T G ->
-    ty_trm m1 m2 G (trm_var (avar_f x)) T
-| ty_all_intro : forall L m1 m2 G T t U,
+    ty_trm m1 m2 G S (trm_var (avar_f x)) T
+| ty_loc : forall m1 m2 G S l T,
+    binds l T S ->
+    ty_trm m1 m2 G S (trm_val (val_loc l)) (typ_ref T)
+| ty_all_intro : forall L m1 m2 G S T t U,
     (forall x, x \notin L ->
-      ty_trm ty_general sub_general (G & x ~ T) (open_trm x t) (open_typ x U)) ->
-    ty_trm m1 m2 G (trm_val (val_lambda T t)) (typ_all T U)
-| ty_all_elim : forall m2 G x z S T,
-    ty_trm ty_general m2 G (trm_var (avar_f x)) (typ_all S T) ->
-    ty_trm ty_general m2 G (trm_var (avar_f z)) S ->
-    ty_trm ty_general m2 G (trm_app (avar_f x) (avar_f z)) (open_typ z T)
-| ty_new_intro : forall L m1 m2 G T ds,
+      ty_trm ty_general sub_general (G & x ~ T) S (open_trm x t) (open_typ x U)) ->
+    ty_trm m1 m2 G S (trm_val (val_lambda T t)) (typ_all T U)
+| ty_all_elim : forall m2 G S x z V T,
+    ty_trm ty_general m2 G S (trm_var (avar_f x)) (typ_all V T) ->
+    ty_trm ty_general m2 G S (trm_var (avar_f z)) V ->
+    ty_trm ty_general m2 G S (trm_app (avar_f x) (avar_f z)) (open_typ z T)
+| ty_new_intro : forall L m1 m2 G S T ds,
     (forall x, x \notin L ->
-      ty_defs (G & (x ~ open_typ x T)) (open_defs x ds) (open_typ x T)) ->
-    ty_trm m1 m2 G (trm_val (val_new T ds)) (typ_bnd T)
-| ty_new_elim : forall m2 G x m T,
-    ty_trm ty_general m2 G (trm_var (avar_f x)) (typ_rcd (dec_trm m T)) ->
-    ty_trm ty_general m2 G (trm_sel (avar_f x) m) T
-| ty_let : forall L m2 G t u T U,
-    ty_trm ty_general m2 G t T ->
+      ty_defs (G & x ~ (open_typ x T)) S (open_defs x ds) (open_typ x T)) ->
+    ty_trm m1 m2 G S (trm_val (val_new T ds)) (typ_bnd T)
+| ty_new_elim : forall m2 G S x m T,
+    ty_trm ty_general m2 G S (trm_var (avar_f x)) (typ_rcd (dec_trm m T)) ->
+    ty_trm ty_general m2 G S (trm_sel (avar_f x) m) T
+| ty_let : forall L m2 G S t u T U,
+    ty_trm ty_general m2 G S t T ->
     (forall x, x \notin L ->
-      ty_trm ty_general sub_general (G & x ~ T) (open_trm x u) U) ->
-    ty_trm ty_general m2 G (trm_let t u) U
-| ty_rec_intro : forall m2 G x T,
-    ty_trm ty_general m2 G (trm_var (avar_f x)) (open_typ x T) ->
-    ty_trm ty_general m2 G (trm_var (avar_f x)) (typ_bnd T)
-| ty_rec_elim : forall m1 m2 G x T,
-    ty_trm m1 m2 G (trm_var (avar_f x)) (typ_bnd T) ->
-    ty_trm m1 m2 G (trm_var (avar_f x)) (open_typ x T)
-| ty_and_intro : forall m2 G x T U,
-    ty_trm ty_general m2 G (trm_var (avar_f x)) T ->
-    ty_trm ty_general m2 G (trm_var (avar_f x)) U ->
-    ty_trm ty_general m2 G (trm_var (avar_f x)) (typ_and T U)
-| ty_sub : forall m2 G t T U,
-    ty_trm ty_general m2 G t T ->
-    subtyp m2 G T U ->
-    ty_trm ty_general m2 G t U
-| ty_and1 : forall m2 G x T U,
-    ty_trm ty_precise m2 G (trm_var (avar_f x)) (typ_and T U) ->
-    ty_trm ty_precise m2 G (trm_var (avar_f x)) T
-| ty_and2 : forall m2 G x T U,
-    ty_trm ty_precise m2 G (trm_var (avar_f x)) (typ_and T U) ->
-    ty_trm ty_precise m2 G (trm_var (avar_f x)) U
-
-with ty_def : ctx -> def -> dec -> Prop :=
-| ty_def_typ : forall G A T,
-    ty_def G (def_typ A T) (dec_typ A T T)
-| ty_def_trm : forall G a t T,
-    ty_trm ty_general sub_general G t T ->
-    ty_def G (def_trm a t) (dec_trm a T)
-with ty_defs : ctx -> defs -> typ -> Prop :=
-| ty_defs_one : forall G d D,
-    ty_def G d D ->
-    ty_defs G (defs_cons defs_nil d) (typ_rcd D)
-| ty_defs_cons : forall G ds d T D,
-    ty_defs G ds T ->
-    ty_def G d D ->
+      ty_trm ty_general sub_general (G & x ~ T) S (open_trm x u) U) ->
+    ty_trm ty_general m2 G S (trm_let t u) U
+| ty_rec_intro : forall m2 G S x T,
+    ty_trm ty_general m2 G S (trm_var (avar_f x)) (open_typ x T) ->
+    ty_trm ty_general m2 G S (trm_var (avar_f x)) (typ_bnd T)
+| ty_rec_elim : forall m1 m2 G S x T,
+    ty_trm m1 m2 G S (trm_var (avar_f x)) (typ_bnd T) ->
+    ty_trm m1 m2 G S (trm_var (avar_f x)) (open_typ x T)
+| ty_and_intro : forall m2 G S x T U,
+    ty_trm ty_general m2 G S (trm_var (avar_f x)) T ->
+    ty_trm ty_general m2 G S (trm_var (avar_f x)) U ->
+    ty_trm ty_general m2 G S (trm_var (avar_f x)) (typ_and T U)
+| ty_sub : forall m2 G S t T U,
+    ty_trm ty_general m2 G S t T ->
+    subtyp m2 G S T U ->
+    ty_trm ty_general m2 G S t U
+| ty_and1 : forall m2 G S x T U,
+    ty_trm ty_precise m2 G S (trm_var (avar_f x)) (typ_and T U) ->
+    ty_trm ty_precise m2 G S (trm_var (avar_f x)) T
+| ty_and2 : forall m2 G S x T U,
+    ty_trm ty_precise m2 G S (trm_var (avar_f x)) (typ_and T U) ->
+    ty_trm ty_precise m2 G S (trm_var (avar_f x)) U
+| ty_ref_intro : forall m1 m2 G S x T,
+     ty_trm m1 m2 G S (trm_var (avar_f x)) T ->
+     ty_trm m1 m2 G S (trm_ref (avar_f x) T) (typ_ref T)
+| ty_ref_elim : forall m1 m2 G S x T,
+    ty_trm m1 m2 G S (trm_var (avar_f x)) (typ_ref T) ->
+    ty_trm m1 m2 G S (trm_deref (avar_f x)) T
+| ty_asgn : forall m1 m2 G S x y T,
+    ty_trm m1 m2 G S (trm_var (avar_f x)) (typ_ref T) ->
+    ty_trm m1 m2 G S (trm_var (avar_f y)) T ->
+    ty_trm m1 m2 G S (trm_asg (avar_f x) (avar_f y)) T
+with ty_def : ctx -> sigma -> def -> dec -> Prop :=
+| ty_def_typ : forall G S A T,
+    ty_def G S (def_typ A T) (dec_typ A T T)
+| ty_def_trm : forall G S a t T,
+    ty_trm ty_general sub_general G S t T ->
+    ty_def G S (def_trm a t) (dec_trm a T)
+with ty_defs : ctx -> sigma -> defs -> typ -> Prop :=
+| ty_defs_one : forall G S d D,
+    ty_def G S d D ->
+    ty_defs G S (defs_cons defs_nil d) (typ_rcd D)
+| ty_defs_cons : forall G S ds d T D,
+    ty_defs G S ds T ->
+    ty_def G S d D ->
     defs_hasnt ds (label_of_def d) ->
-    ty_defs G (defs_cons ds d) (typ_and T (typ_rcd D))
+    ty_defs G S (defs_cons ds d) (typ_and T (typ_rcd D))
 
-with subtyp : submode -> ctx -> typ -> typ -> Prop :=
-| subtyp_top: forall m2 G T,
-    subtyp m2 G T typ_top
-| subtyp_bot: forall m2 G T,
-    subtyp m2 G typ_bot T
-| subtyp_refl: forall m2 G T,
-    subtyp m2 G T T
-| subtyp_trans: forall m2 G S T U,
-    subtyp m2 G S T ->
-    subtyp m2 G T U ->
-    subtyp m2 G S U
-| subtyp_and11: forall m2 G T U,
-    subtyp m2 G (typ_and T U) T
-| subtyp_and12: forall m2 G T U,
-    subtyp m2 G (typ_and T U) U
-| subtyp_and2: forall m2 G S T U,
-    subtyp m2 G S T ->
-    subtyp m2 G S U ->
-    subtyp m2 G S (typ_and T U)
-| subtyp_fld: forall m2 G a T U,
-    subtyp m2 G T U ->
-    subtyp m2 G (typ_rcd (dec_trm a T)) (typ_rcd (dec_trm a U))
-| subtyp_typ: forall m2 G A S1 T1 S2 T2,
-    subtyp m2 G S2 S1 ->
-    subtyp m2 G T1 T2 ->
-    subtyp m2 G (typ_rcd (dec_typ A S1 T1)) (typ_rcd (dec_typ A S2 T2))
-| subtyp_sel2: forall G x A S T,
-    ty_trm ty_general sub_general G (trm_var (avar_f x)) (typ_rcd (dec_typ A S T)) ->
-    subtyp sub_general G S (typ_sel (avar_f x) A)
-| subtyp_sel1: forall G x A S T,
-    ty_trm ty_general sub_general G (trm_var (avar_f x)) (typ_rcd (dec_typ A S T)) ->
-    subtyp sub_general G (typ_sel (avar_f x) A) T
-| subtyp_sel2_tight: forall G x A T,
-    ty_trm ty_precise sub_general G (trm_var (avar_f x)) (typ_rcd (dec_typ A T T)) ->
-    subtyp sub_tight G T (typ_sel (avar_f x) A)
-| subtyp_sel1_tight: forall G x A T,
-    ty_trm ty_precise sub_general G (trm_var (avar_f x)) (typ_rcd (dec_typ A T T)) ->
-    subtyp sub_tight G (typ_sel (avar_f x) A) T
-| subtyp_all: forall L m2 G S1 T1 S2 T2,
-    subtyp m2 G S2 S1 ->
+with subtyp : submode -> ctx -> sigma -> typ -> typ -> Prop :=
+(* sigma is not needed for subtyping but for induction *)
+| subtyp_top: forall m2 G S T,
+    subtyp m2 G S T typ_top
+| subtyp_bot: forall m2 G S T,
+    subtyp m2 G S typ_bot T
+| subtyp_refl: forall m2 G S T,
+    subtyp m2 G S T T
+| subtyp_trans: forall m2 G S V T U,
+    subtyp m2 G S V T ->
+    subtyp m2 G S T U ->
+    subtyp m2 G S V U
+| subtyp_and11: forall m2 G S T U,
+    subtyp m2 G S (typ_and T U) T
+| subtyp_and12: forall m2 G S T U,
+    subtyp m2 G S (typ_and T U) U
+| subtyp_and2: forall m2 G S V T U,
+    subtyp m2 G S V T ->
+    subtyp m2 G S V U ->
+    subtyp m2 G S V (typ_and T U)
+| subtyp_fld: forall m2 G S a T U,
+    subtyp m2 G S T U ->
+    subtyp m2 G S (typ_rcd (dec_trm a T)) (typ_rcd (dec_trm a U))
+| subtyp_typ: forall m2 G S A S1 T1 S2 T2,
+    subtyp m2 G S S2 S1 ->
+    subtyp m2 G S T1 T2 ->
+    subtyp m2 G S (typ_rcd (dec_typ A S1 T1)) (typ_rcd (dec_typ A S2 T2))
+| subtyp_sel2: forall G S x A V T,
+    ty_trm ty_general sub_general G S (trm_var (avar_f x)) (typ_rcd (dec_typ A V T)) ->
+    subtyp sub_general G S V (typ_sel (avar_f x) A)
+| subtyp_sel1: forall G S x A V T,
+    ty_trm ty_general sub_general G S (trm_var (avar_f x)) (typ_rcd (dec_typ A V T)) ->
+    subtyp sub_general G S (typ_sel (avar_f x) A) T
+| subtyp_sel2_tight: forall G S x A T,
+    ty_trm ty_precise sub_general G S (trm_var (avar_f x)) (typ_rcd (dec_typ A T T)) ->
+    subtyp sub_tight G S T (typ_sel (avar_f x) A)
+| subtyp_sel1_tight: forall G S x A T,
+    ty_trm ty_precise sub_general G S (trm_var (avar_f x)) (typ_rcd (dec_typ A T T)) ->
+    subtyp sub_tight G S (typ_sel (avar_f x) A) T
+| subtyp_all: forall L m2 G S S1 T1 S2 T2,
+    subtyp m2 G S S2 S1 ->
     (forall x, x \notin L ->
-       subtyp sub_general (G & x ~ S2) (open_typ x T1) (open_typ x T2)) ->
-    subtyp m2 G (typ_all S1 T1) (typ_all S2 T2).
+       subtyp sub_general (G & x ~ S2) S (open_typ x T1) (open_typ x T2)) ->
+    subtyp m2 G S (typ_all S1 T1) (typ_all S2 T2)
+| subtyp_ref: forall m2 G S T U,
+    subtyp m2 G S T U ->
+    subtyp m2 G S U T ->
+    subtyp m2 G S (typ_ref T) (typ_ref U).
 
-Inductive wf_sto: ctx -> sto -> Prop :=
-| wf_sto_empty: wf_sto empty empty
-| wf_sto_push: forall G s x T v,
-    wf_sto G s ->
+(* well-formed stack *)
+Inductive wf_stack: ctx -> sigma -> stack -> Prop :=
+| wf_stack_empty: wf_stack empty empty empty
+| wf_stack_push: forall G S sta x T v,
+    wf_stack G S sta ->
     x # G ->
-    x # s ->
-    ty_trm ty_general sub_general G (trm_val v) T ->
-    wf_sto (G & x ~ T) (s & x ~ v).
+    x # sta ->
+    ty_trm ty_general sub_general G S (trm_val v) T ->
+    wf_stack (G & x ~ T) S (sta & x ~ v)
+| wf_store_push: forall G S l T sta,
+    wf_stack G S sta ->
+    l # S ->
+    wf_stack G (S & l ~ T) sta.
+
+(* well-typed store *)
+Inductive wt_store: ctx -> sigma -> store -> Prop :=
+| wt_store_empty: wt_store empty empty emptyM
+| wt_store_update: forall G S sto l x T,
+    wt_store G S sto ->
+    binds l T S ->
+    ty_trm ty_general sub_general G S (trm_var (avar_f x)) T ->
+    wt_store G S sto[l := x]
+| wt_store_new: forall G S sto l x T,
+    wt_store G S sto ->
+    l # S ->
+    ty_trm ty_general sub_general G S (trm_var (avar_f x)) T ->
+    wt_store G (S & l ~ T) sto[l := x]
+| wt_stack_push: forall G S x T sto,
+    wt_store G S sto ->
+    x # G ->
+    wt_store (G & x ~ T) S sto.
 
 (* ###################################################################### *)
 (* ###################################################################### *)
@@ -395,14 +455,19 @@ with   def_mut  := Induction for def  Sort Prop
 with   defs_mut := Induction for defs Sort Prop.
 Combined Scheme trm_mutind from trm_mut, val_mut, def_mut, defs_mut.
 
+Scheme ty_trm_mut    := Induction for ty_trm    Sort Prop
+with   ty_def_mut    := Induction for ty_def    Sort Prop
+with   ty_defs_mut   := Induction for ty_defs   Sort Prop.
+Combined Scheme ty_mutind from ty_trm_mut, ty_def_mut, ty_defs_mut.
+
 Scheme ts_ty_trm_mut := Induction for ty_trm    Sort Prop
-with   ts_subtyp     := Induction for subtyp    Sort Prop.
+with   ts_subtyp    := Induction for subtyp   Sort Prop.
 Combined Scheme ts_mutind from ts_ty_trm_mut, ts_subtyp.
 
 Scheme rules_trm_mut    := Induction for ty_trm    Sort Prop
 with   rules_def_mut    := Induction for ty_def    Sort Prop
 with   rules_defs_mut   := Induction for ty_defs   Sort Prop
-with   rules_subtyp     := Induction for subtyp    Sort Prop.
+with   rules_subtyp    := Induction for subtyp   Sort Prop.
 Combined Scheme rules_mutind from rules_trm_mut, rules_def_mut, rules_defs_mut, rules_subtyp.
 
 (* ###################################################################### *)
@@ -411,15 +476,16 @@ Combined Scheme rules_mutind from rules_trm_mut, rules_def_mut, rules_defs_mut, 
 Ltac gather_vars :=
   let A := gather_vars_with (fun x : vars      => x         ) in
   let B := gather_vars_with (fun x : var       => \{ x }    ) in
-  let C := gather_vars_with (fun x : ctx       => (dom x) \u (fv_ctx_types x)) in
-  let D := gather_vars_with (fun x : sto       => dom x     ) in
-  let E := gather_vars_with (fun x : avar      => fv_avar  x) in
-  let F := gather_vars_with (fun x : trm       => fv_trm   x) in
-  let G := gather_vars_with (fun x : val       => fv_val   x) in
-  let H := gather_vars_with (fun x : def       => fv_def   x) in
-  let I := gather_vars_with (fun x : defs      => fv_defs  x) in
-  let J := gather_vars_with (fun x : typ       => fv_typ   x) in
-  constr:(A \u B \u C \u D \u E \u F \u G \u H \u I \u J).
+  let C := gather_vars_with (fun x : ctx       => (dom x) \u (fv_env_types x)) in
+  let D := gather_vars_with (fun x : sigma     => (dom x) \u (fv_env_types x)) in
+  let E := gather_vars_with (fun x : stack     => dom x     ) in
+  let F := gather_vars_with (fun x : avar      => fv_avar  x) in
+  let G := gather_vars_with (fun x : trm       => fv_trm   x) in
+  let H := gather_vars_with (fun x : val       => fv_val   x) in
+  let I := gather_vars_with (fun x : def       => fv_def   x) in
+  let J := gather_vars_with (fun x : defs      => fv_defs  x) in
+  let K := gather_vars_with (fun x : typ       => fv_typ   x) in
+  constr:(A \u B \u C \u D \u E \u F \u G \u H \u I \u J \u K).
 
 Ltac pick_fresh x :=
   let L := gather_vars in (pick_fresh_gen L x).
@@ -443,12 +509,11 @@ Ltac crush := eq_specialize; eauto.
 Tactic Notation "apply_fresh" constr(T) "as" ident(x) :=
   apply_fresh_base T gather_vars x.
 
-(* todo: add constructor hints for the new typing relations *)
 Hint Constructors
   ty_trm ty_def ty_defs
   subtyp.
 
-Hint Constructors wf_sto.
+Hint Constructors wf_stack wt_store.
 
 Hint Constructors record_has.
 
