dev/lf/tight-proof/Canonical_forms1.v
@@ -16,43 +16,46 @@ Lemma (Canonical forms 1)
 If G ~ s and G |- x: all(x: T)U then s(x) = lambda(x: T')t where G |- T <: T' and G, x: T |- t: U.
  *)
 
-Lemma canonical_forms_1: forall G s x T U,
-  wf_sto G s ->
+Lemma canonical_forms_1: forall G S s x T U,
+  wf_stack G S s ->
   inert G ->
-  ty_trm ty_general sub_general G (trm_var (avar_f x)) (typ_all T U) ->
-  (exists L T' t, binds x (val_lambda T' t) s /\ subtyp sub_general G T T' /\
-  (forall y, y \notin L -> ty_trm ty_general sub_general (G & y ~ T) (open_trm y t) (open_typ y U))).
+  ty_trm ty_general sub_general G S (trm_var (avar_f x)) (typ_all T U) ->
+  (exists L T' t, 
+      binds x (val_lambda T' t) s /\ 
+      subtyp sub_general G S T T' /\
+      (forall y, y \notin L -> ty_trm ty_general sub_general (G & y ~ T) S (open_trm y t) (open_typ y U))).
 Proof.
   introv Hwf Hgd Hty.
   pose proof (general_to_tight_typing Hgd Hty) as Hti.
-  pose proof (tight_to_precise_typ_all Hgd Hti) as [S' [T' [L' [Hpt [HSsub HTsub]]]]].
+  pose proof (tight_to_precise_typ_all Hgd Hti) as [T' [U' [L' [Hpt [HSsub HTsub]]]]].
   pose proof (inert_precise_all_inv Hgd Hpt) as Bi.
   pose proof (corresponding_types Hwf Hgd Bi)
-    as [[L [S [V [S1 [V1 [t [Hb [Ht [Heq [Hs1 Hs2]]]]]]]]]] | [S [ds [Hb [Ht Heq]]]]].
+    as [[L [V [W [V1 [W1 [t [Hb [Ht [Heq [Hs1 Hs2]]]]]]]]]] | [[V [ds [Hb [Ht Heq]]]] | [V [V' [l [Hb [Ht [Heq [Hs1 Hs2]]]]]]]]].
   subst. inversion Heq; subst. inversions Ht.
-  - exists (L \u L' \u L0 \u dom G) S t.
+  - exists (L \u L' \u L0 \u dom G) V t.
     split; auto.
     pose proof (tight_possible_types_lemma Hgd Hti) as Htp.
     assert (forall y W, y # G -> ok (G & y ~ W)) as Hok by (intros; apply* ok_push).
     inversion Htp; subst.
     + apply (inert_precise_all_inv Hgd) in Hpt.
       apply (inert_precise_all_inv Hgd) in H.
-      pose proof (binds_func Hpt H) as H4.
-      inversion H4; subst T U; clear H4.
+      pose proof (binds_func Hpt H) as H5.
+      inversion H5; subst T U; clear H5.
       split. auto. intros y Hy.
       assert (y \notin L0) as Hy0 by auto. assert (y \notin L) as HyL by auto.
-      specialize (H3 y Hy0). apply narrow_typing with (G':=G & y ~ S1) in H3.
-      apply ty_sub with (T:=open_typ y V).
+      specialize (H4 y Hy0). apply narrow_typing with (G':=G & y ~ V1) in H4.
+      apply ty_sub with (T:=open_typ y W).
       assumption. apply* Hs2. apply* subenv_last. apply* Hok.
     + apply tight_to_general in HSsub; auto.
-      assert (subtyp sub_general G T S) as HTS by (apply* subtyp_trans).
+      assert (subtyp sub_general G S T V) as HTV by (apply* subtyp_trans).
       split; auto. intros y Hy. assert (y \notin L0) as Hy0 by auto.
-      specialize (H3 y Hy0).
-      apply narrow_typing with (G':=G & y ~ T) in H3. apply ty_sub with (T:=open_typ y V).
-      assumption. apply subtyp_trans with (T:=open_typ y V1).
+      specialize (H4 y Hy0).
+      apply narrow_typing with (G':=G & y ~ T) in H4. apply ty_sub with (T:=open_typ y W).
+      assumption. apply subtyp_trans with (T:=open_typ y W1).
       assert (y \notin L) as HL by auto.
       specialize (Hs2 y HL). apply narrow_subtyping with (G':=G & y ~ T) in Hs2.
       assumption. apply* subenv_last. apply* Hok.
       apply* HTsub. apply* subenv_last. apply* Hok.
+  - inversion Heq.
   - inversion Heq.
 Qed.
