dev/lf/tight-proof/Safety.v
@@ -1,6 +1,6 @@
 Set Implicit Arguments.
 
-Require Import LibLN.
+Require Import LibMap LibLN.
 Require Import Coq.Program.Equality.
 Require Import Definitions.
 Require Import Weakening.
@@ -10,6 +10,7 @@ Require Import Narrowing.
 Require Import Some_lemmas.
 Require Import Canonical_forms1.
 Require Import Canonical_forms2.
+Require Import Canonical_forms3.
 Require Import Inert_types.
 Require Import General_to_tight.
 
@@ -34,38 +35,49 @@ Let G |- t: T and G ~ s. Then either
 The proof is by a induction on typing derivations of G |- t: T.
 *)
 
-Lemma safety: forall G s t T,
-    wf_sto G s ->
+Lemma safety: forall G S sta sto t T,
+    wf_stack G S sta ->
+    wt_store G S sto ->
     inert G ->
-    ty_trm ty_general sub_general G t T ->
-    (normal_form t \/ (exists s' t' G' G'', red t s t' s' /\ G' = G & G'' /\ ty_trm ty_general sub_general G' t' T /\ wf_sto G' s')).
+    ty_trm ty_general sub_general G S t T ->
+    (normal_form t \/ 
+      (exists sta' sto' t' G' G'' S' S'',
+      red t sta sto t' sta' sto' /\ 
+      G' = G & G'' /\ 
+      S' = S & S'' /\
+      ty_trm ty_general sub_general G' S' t' T /\ 
+      wf_stack G' S' sta' /\
+      wt_store G' S' sto')).
 Proof.
-  introv Hwf Hg H. dependent induction H; try solve [left; eauto].
-  - (* All-E *) right.
+  introv Hwf Hwt Hg H. dependent induction H; try solve [left; eauto].
+  - (* All-E *) 
+    right.
     lets C: (canonical_forms_1 Hwf Hg H).
     destruct C as [L [T' [t [Bis [Hsub Hty]]]]].
-    exists s (open_trm z t) G (@empty typ).
-    split.
-    apply red_app with (T:=T'). assumption.
-    split.
-    rewrite concat_empty_r. reflexivity.
-    split.
-    pick_fresh y. assert (y \notin L) as FrL by auto. specialize (Hty y FrL).
-    rewrite subst_intro_typ with (x:=y). rewrite subst_intro_trm with (x:=y).
-    eapply subst_ty_trm. eapply Hty.
-    apply ok_push. eapply wf_sto_to_ok_G. eassumption. eauto. eauto.
-    rewrite subst_fresh_typ.
-    apply ty_sub with (T:=S).
-    assumption. apply subtyp_refl.
-    eauto. eauto. eauto. eauto.
+    exists sta sto (open_trm z t) G (@empty typ). exists S (@empty typ).
+    repeat split.
+    + apply red_app with (T:=T'). assumption.
+    + rewrite concat_empty_r. reflexivity.
+    + rewrite concat_empty_r. reflexivity.
+    + pick_fresh y. assert (y \notin L) as FrL by auto. specialize (Hty y FrL).
+      rewrite subst_intro_typ with (x:=y); auto. rewrite subst_intro_trm with (x:=y); auto.
+      eapply subst_ty_trm; auto.
+      * eapply Hty.
+      * apply* ok_push. 
+      * rewrite* subst_fresh_typ.
+    + assumption. 
+    + assumption. 
   - (* Fld-E *) right.
-    pose proof (canonical_forms_2 Hg Hwf H) as [S [ds [t [Bis [Has Ty]]]]].
-    exists s t G (@empty typ).
+    pose proof (canonical_forms_2 Hg Hwf H) as [V [ds [t [Bis [Has Ty]]]]].
+    exists sta sto t G (@empty typ). exists S (@empty typ).
     split.
-    + apply red_sel with (T:=S) (ds:=ds); assumption.
-    + split.
+    + apply red_sel with (T:=V) (ds:=ds); assumption.
+    + repeat split.
       * rewrite concat_empty_r. reflexivity.
-      * split; assumption.
+      * rewrite concat_empty_r. reflexivity.
+      * assumption.
+      * assumption.
+      * assumption.
   - (* Let *) right.
     destruct t.
     + (* var *)
@@ -73,61 +85,168 @@ Proof.
         eapply var_typing_implies_avar_f. eassumption.
       }
       destruct A as [x A]. subst a.
-      exists s (open_trm x u) G (@empty typ).
-      split.
-      apply red_let_var.
-      split.
-      rewrite concat_empty_r. reflexivity.
-      split.
-      pick_fresh y. assert (y \notin L) as FrL by auto. specialize (H0 y FrL).
-      rewrite subst_intro_trm with (x:=y).
-      rewrite <- subst_fresh_typ with (x:=y) (y:=x).
-      eapply subst_ty_trm. eapply H0.
-      apply ok_push. eapply wf_sto_to_ok_G. eassumption. eauto. eauto.
-      rewrite subst_fresh_typ. assumption. eauto. eauto. eauto. eauto.
+      exists sta sto (open_trm x u) G (@empty typ). exists S (@empty typ).
+      repeat split.
+      * apply red_let_var.
+      * rewrite concat_empty_r. reflexivity.
+      * rewrite concat_empty_r. reflexivity.
+      * pick_fresh y. assert (y \notin L) as FrL by auto. specialize (H0 y FrL).
+        rewrite subst_intro_trm with (x:=y); auto.
+        rewrite <- subst_fresh_typ with (x:=y) (y:=x); auto.
+        eapply subst_ty_trm; auto. eapply H0.
+        apply* ok_push.
+        rewrite* subst_fresh_typ. 
+      * assumption.
+      * assumption.
     + lets Hv: (val_typing H).
       destruct Hv as [T' [Htyp Hsub]].
       pick_fresh x. assert (x \notin L) as FrL by auto. specialize (H0 x FrL).
-      exists (s & x ~ v) (open_trm x u) (G & x ~ T) (x ~ T).
-      split.
-      apply red_let. eauto.
-      split. reflexivity. split. assumption. apply* wf_sto_push.
+      exists (sta & x ~ v) sto (open_trm x u) (G & x ~ T) (x ~ T). exists S (@empty typ).
+      repeat split.
+      * apply* red_let. 
+      * rewrite concat_empty_r. reflexivity. 
+      * assumption. 
+      * apply* wf_stack_push.
+      * apply* wt_stack_push.
     + specialize (IHty_trm Hwf). destruct IHty_trm as [IH | IH]; auto. inversion IH.
-      destruct IH as [s' [t' [G' [G'' [IH1 [IH2 [IH3]]]]]]].
-      exists s' (trm_let t' u) G' G''.
-      split. apply red_let_tgt. assumption.
-      split. assumption. split.
-      apply ty_let with (L:=L \u dom G') (T:=T); eauto.
-      intros. rewrite IH2. eapply (proj51 weaken_rules). apply H0. auto. reflexivity.
-      rewrite <- IH2. apply ok_push. eapply wf_sto_to_ok_G. eassumption. eauto.
-      rewrite IH2.
-      rewrite <- IH2. eauto.
+      destruct IH as [sta' [sto' [t' [G' [G'' [S' [S'' [IH1 [IH2 [IH3 [IH4 [IH5 IH6]]]]]]]]]]]].
+      exists sta' sto' (trm_let t' u) G' G''. exists S' S''.
+      repeat split. 
+      * apply red_let_tgt. assumption.
+      * assumption. 
+      * assumption.
+      * apply ty_let with (L:=L \u dom G') (T:=T); eauto. intros.
+        rewrite IH3. apply weaken_ty_trm_sigma. 
+        rewrite IH2. eapply (proj41 weaken_rules_ctx). 
+        apply H0. auto. reflexivity.
+        rewrite <- IH2. apply ok_push. eapply wf_stack_to_ok_G. eassumption. eauto.
+        eapply wf_stack_to_ok_S. subst. eauto.
+      * rewrite IH2. rewrite <- IH2. eauto.
+      * assumption.
     + specialize (IHty_trm Hwf). destruct IHty_trm as [IH | IH]; auto. inversion IH.
-      destruct IH as [s' [t' [G' [G'' [IH1 [IH2 [IH3]]]]]]].
-      exists s' (trm_let t' u) G' G''.
-      split. apply red_let_tgt. assumption.
-      split. assumption. split.
-      apply ty_let with (L:=L \u dom G') (T:=T); eauto.
-      intros. rewrite IH2. eapply (proj51 weaken_rules). apply H0. auto. reflexivity.
-      rewrite <- IH2. apply ok_push. eapply wf_sto_to_ok_G. eassumption. eauto.
-      rewrite IH2.
-      rewrite <- IH2. eauto.
+      destruct IH as [sta' [sto' [t' [G' [G'' [S' [S'' [IH1 [IH2 [IH3 [IH4 [IH5 IH6]]]]]]]]]]]].
+      exists sta' sto' (trm_let t' u) G' G''. exists S' S''.
+      repeat split. 
+      * apply red_let_tgt. assumption.
+      * assumption. 
+      * assumption.
+      * apply ty_let with (L:=L \u dom G') (T:=T); eauto. intros.
+        rewrite IH3. apply weaken_ty_trm_sigma.
+        rewrite IH2. eapply (proj41 weaken_rules_ctx). apply H0. auto. 
+        reflexivity.
+        rewrite <- IH2. apply ok_push. eapply wf_stack_to_ok_G. eassumption. 
+        eauto. eapply wf_stack_to_ok_S. subst. eauto.
+      * rewrite IH2. rewrite <- IH2. eauto.
+      * assumption.
     + specialize (IHty_trm Hwf). destruct IHty_trm as [IH | IH]; auto. inversion IH.
-      destruct IH as [s' [t' [G' [G'' [IH1 [IH2 [IH3]]]]]]].
-      exists s' (trm_let t' u) G' G''.
-      split. apply red_let_tgt. assumption.
-      split. assumption. split.
-      apply ty_let with (L:=L \u dom G') (T:=T); eauto.
-      intros. rewrite IH2. eapply (proj51 weaken_rules). apply H0. auto. reflexivity.
-      rewrite <- IH2. apply ok_push. eapply wf_sto_to_ok_G. eassumption. eauto.
-      rewrite IH2.
-      rewrite <- IH2. eauto.
+      destruct IH as [sta' [sto' [t' [G' [G'' [S' [S'' [IH1 [IH2 [IH3 [IH4 [IH5 IH6]]]]]]]]]]]].
+      exists sta' sto' (trm_let t' u) G' G''. exists S' S''.
+      repeat split. 
+      * apply red_let_tgt. assumption.
+      * assumption. 
+      * assumption. 
+      * apply ty_let with (L:=L \u dom G') (T:=T); eauto. intros. 
+        rewrite IH3. apply weaken_ty_trm_sigma.
+        rewrite IH2. eapply (proj41 weaken_rules_ctx). apply H0. auto. 
+        reflexivity.
+        rewrite <- IH2. apply ok_push. eapply wf_stack_to_ok_G. eassumption. 
+        eauto. eapply wf_stack_to_ok_S. subst. eauto.
+      * assumption.
+      * assumption.
+    + specialize (IHty_trm Hwf). destruct IHty_trm as [IH | IH]; auto. inversion IH.
+      destruct IH as [sta' [sto' [t' [G' [G'' [S' [S'' [IH1 [IH2 [IH3 [IH4 [IH5 IH6]]]]]]]]]]]].
+      exists sta' sto' (trm_let t' u) G' G''. exists S' S''.
+      repeat split. 
+      * apply red_let_tgt. assumption.
+      * assumption. 
+      * assumption. 
+      * apply ty_let with (L:=L \u dom G') (T:=T); eauto. intros. 
+        rewrite IH3. apply weaken_ty_trm_sigma.
+        rewrite IH2. eapply (proj41 weaken_rules_ctx). apply H0. auto. 
+        reflexivity.
+        rewrite <- IH2. apply ok_push. eapply wf_stack_to_ok_G. eassumption. 
+        eauto. eapply wf_stack_to_ok_S. subst. eauto.
+      * assumption.
+      * assumption.
+    + specialize (IHty_trm Hwf). destruct IHty_trm as [IH | IH]; auto. inversion IH.
+      destruct IH as [sta' [sto' [t' [G' [G'' [S' [S'' [IH1 [IH2 [IH3 [IH4 [IH5 IH6]]]]]]]]]]]].
+      exists sta' sto' (trm_let t' u) G' G''. exists S' S''.
+      repeat split. 
+      * apply red_let_tgt. assumption.
+      * assumption. 
+      * assumption. 
+      * apply ty_let with (L:=L \u dom G') (T:=T); eauto. intros. 
+        rewrite IH3. apply weaken_ty_trm_sigma.
+        rewrite IH2. eapply (proj41 weaken_rules_ctx). apply H0. auto. 
+        reflexivity.
+        rewrite <- IH2. apply ok_push. eapply wf_stack_to_ok_G. eassumption. 
+        eauto. eapply wf_stack_to_ok_S. subst. eauto.
+      * assumption.
+      * assumption.
+    + specialize (IHty_trm Hwf). destruct IHty_trm as [IH | IH]; auto. inversion IH.
+      destruct IH as [sta' [sto' [t' [G' [G'' [S' [S'' [IH1 [IH2 [IH3 [IH4 [IH5 IH6]]]]]]]]]]]].
+      exists sta' sto' (trm_let t' u) G' G''. exists S' S''.
+      repeat split. 
+      * apply red_let_tgt. assumption.
+      * assumption. 
+      * assumption. 
+      * apply ty_let with (L:=L \u dom G') (T:=T); eauto. intros. 
+        rewrite IH3. apply weaken_ty_trm_sigma.
+        rewrite IH2. eapply (proj41 weaken_rules_ctx). apply H0. auto. 
+        reflexivity.
+        rewrite <- IH2. apply ok_push. eapply wf_stack_to_ok_G. eassumption. 
+        eauto. eapply wf_stack_to_ok_S. subst. eauto.
+      * assumption.
+      * assumption.
   - specialize (IHty_trm Hwf). destruct IHty_trm as [IH | IH]; auto.
-    right. destruct IH as [s' [t' [G' [G'' [IH1 [IH2 [IH3]]]]]]].
-    exists s' t' G' G''.
-    split; try split; try split; try assumption.
+    right. destruct IH as [sta' [sto' [t' [G' [G'' [S' [S'' [IH1 [IH2 [IH3 [IH4 [IH5 IH6]]]]]]]]]]]].
+    exists sta' sto' t' G' G''. exists S' S''.
+    split; try split; try split; try split; try split; try assumption.
     apply ty_sub with (T:=T).
     assumption.
-    rewrite IH2. apply weaken_subtyp. assumption.
-    rewrite <- IH2. eapply wf_sto_to_ok_G. eassumption.
+    rewrite IH3. apply weaken_subtyp_sigma.
+    rewrite IH2. apply weaken_subtyp_ctx. assumption.
+    rewrite <- IH2. eapply wf_stack_to_ok_G. eassumption.
+    rewrite <- IH3. eapply wf_stack_to_ok_S. eassumption.
+  - (* ref *)
+    right. pick_fresh l.
+    exists sta (sto[l:=x]) (trm_val (val_loc l)) G (@empty typ). exists (S & l ~ T) (l ~ T).
+    split. apply* red_ref_var.
+    assert (l # S) as HS by auto.
+    apply (wt_notin_dom Hwt HS).
+    split. rewrite concat_empty_r. reflexivity.
+    split. reflexivity.
+    split. constructor. auto.
+    split. constructor. assumption. auto.
+    apply wt_store_new. assumption. auto.
+    assumption. 
+  - (* deref *)
+    right.
+    lets C: (canonical_forms_3 Hg Hwf Hwt H).
+    destruct C as [l [y [BiLoc [_ [BiVal Htyval]]]]].
+    exists sta sto (trm_var (avar_f y)) G (@empty typ). exists S (@empty typ).
+    split. apply red_deref with (l:=l). assumption. assumption.
+    split. rewrite concat_empty_r. reflexivity.
+    split. rewrite concat_empty_r. reflexivity.
+    split. assumption. split. assumption. assumption.
+  - (* asg *)
+    right.
+    pose proof (canonical_forms_3 Hg Hwf Hwt H) as [l [y' [BiLoc [Hty [BiSto Htyy']]]]].
+    exists sta (sto[l := y]) (trm_var (avar_f y)) G (@empty typ). exists S (@empty typ).
+    split.
+    + apply red_asgn with (l:=l).
+      * assumption.
+      * lets Hbd: (LibMap.binds_def sto l y'). unfold bindsM in BiSto. rewrite Hbd in BiSto.
+        destruct BiSto as [His Hsto]. assumption.
+    + repeat split.
+      * rewrite concat_empty_r. reflexivity.
+      * rewrite concat_empty_r. reflexivity.
+      * assumption.
+      * assumption.
+      * pose proof (general_to_tight Hg) as [A _].
+        pose proof (A ty_general sub_general G S (trm_var (avar_f x)) (typ_ref T) H eq_refl eq_refl eq_refl).
+        pose proof (A ty_general sub_general G S (trm_val (val_loc l)) (typ_ref T) Hty eq_refl eq_refl eq_refl).
+        destruct (precise_ref_subtyping Hg BiLoc H1 H2 Hwf Hwt) as [U [HU [Hs1 Hs2]]].
+        apply wt_store_update with (T:=U); try assumption.
+        apply (ref_binds_typ HU). apply ty_sub with (T:=T); assumption.
 Qed.
